new/extract.v
@@ -1,3 +1,12 @@
-Require Import insert copy.
+Require Import insert copy Arith.Div2 Arith.Even.
 
-Recursive Extraction insert.insert copy.copy.
+Extract Inductive bool => "bool" [ "false" "true" ].
+Extract Inductive sumbool => "bool" [ "false" "true" ].
+Extract Inductive prod => "(*)"  [ "(,)" ].
+Extract Inductive nat => 
+"int" [ "0" "succ" ]
+      "(fun fO fS n -> if n=0 then fO () else fS (n-1))".
+Extract Constant div2 => "fun a -> a / 2".
+Extract Constant even_odd_dec => "fun a -> (a mod 2) != 0".
+
+Extraction "braun.ml" insert.insert copy.copy.
